src/xor/direct_xor.lean
@@ -21,29 +21,29 @@ universe u
 -- Represents the parametric type of the variable stored in the literal
 variables {V : Type u} [decidable_eq V] [inhabited V]
 
-namespace xor_gate
+namespace nxor
 
 open literal
 open clause -- TODO opening clause doesn't seem to open library...
 open cnf
 open list
-open xor_gate
+open nxor
 open explode
 open nat
 
 /-! # Direct encoding -/
 section direct_encoding
 
-variables {g : xor_gate V} {c : clause V}
+variables {g : nxor V} {c : clause V}
 
 /- The direct encoding is the set of all possible clauses with an even number 
    of negations on the provided literals in a single CNF formula. -/
-def direct_xor : xor_gate V → cnf V
+def direct_xor : nxor V → cnf V
 | []        := [[]]
 | (l :: ls) := (explode (map var ls)).map 
       (λ c, cond (bodd (c.count_flips (ls)) = ff) (l :: c) (l.flip :: c))
 
-@[simp] theorem direct_xor_nil : direct_xor ([] : xor_gate V) = [[]] := rfl
+@[simp] theorem direct_xor_nil : direct_xor ([] : nxor V) = [[]] := rfl
 
 @[simp] theorem direct_xor_singleton (l : literal V) : direct_xor [l] = [[l]] :=
 by simp [direct_xor]
@@ -77,7 +77,7 @@ end
 theorem length_direct_xor_pos : g ≠ [] → length (direct_xor g) > 0 :=
 assume h, by simp only [length_direct_xor h, succ_pos', gt_iff_lt, pow_pos]
 
-theorem exists_mem_direct_xor (g : xor_gate V) : 
+theorem exists_mem_direct_xor (g : nxor V) : 
   ∃ (c : clause V), c ∈ direct_xor g :=
 begin
   cases g with l ls,
@@ -86,7 +86,7 @@ begin
 end
 
 -- These theorems begin to be dependent on order of encoding
--- If the underlying type of xor_gate changes to (fin)set, must update
+-- If the underlying type of nxor changes to (fin)set, must update
 theorem map_var_eq_of_mem_direct_xor :
   c ∈ direct_xor g → map var c = map var g :=
 begin
@@ -145,43 +145,14 @@ begin
     exact (even_flips_iff_mem_direct_xor_of_map_var_eq hc).mp }
 end
 
-theorem direct_xor_equisatisfiable (g : xor_gate V) :
-  assignment.eqsat (λ α, cnf.eval α (direct_xor g)) (λ α, g.eval α) :=
-begin
-  split,
-  { rintros ⟨α, ha⟩, use α,
-    simp [eval_eq_bodd_count_tt α g],
-    simp at ha,
-    rcases exists_mem_direct_xor g with ⟨c, hc⟩,
-    by_contradiction,
-    rw [eq_ff_eq_not_eq_tt, ← clause.count_flips_falsify_eq_count_tt, 
-      clause.count_flips_comm] at h,
-    have falsify_mem := (even_flips_iff_mem_direct_xor_of_map_var_eq 
-      (clause.falsify_map_var_eq α (map var g))).mp h,
-    have falsify_eval := clause.falsify_eval_ff α (map var g),
-    have := eval_tt_iff_forall_clause_eval_tt.mp ha,
-    rw this (clause.falsify α (map var g)) falsify_mem at falsify_eval,
-    contradiction },
-  { rintros ⟨α, ha⟩, use α,
-    simp [eval_eq_bodd_count_tt] at ha,
-    apply eval_tt_iff_forall_clause_eval_tt.mpr,
-    intros c hc,
-    have mve := map_var_eq_of_mem_direct_xor hc,
-    have := (even_flips_iff_mem_direct_xor_of_map_var_eq mve).mpr hc,
-    have neqodd := ne_of_eq_ff_of_eq_tt this ha,
-    have neq := ne_of_apply_ne nat.bodd neqodd,
-    rw clause.count_flips_comm at neq,
-    exact clause.eval_tt_of_neq_flips mve.symm (ne.symm neq) }
-end
-
 -- Some proofs require the stronger statement that direct is exactly xor
-theorem eval_direct_xor_eq_eval_xor_gate (g : xor_gate V) (α : assignment V) :
+theorem eval_direct_xor_eq_eval_nxor (g : nxor V) (α : assignment V) :
   cnf.eval α (direct_xor g) = g.eval α :=
 begin
   cases g with l ls,
   { simp only [cnf.eval_singleton, eval_nil, direct_xor_nil, clause.eval_nil] },
   { have he := eval_eq_bodd_count_tt α (l :: ls),
-    cases h : (xor_gate.eval α (l :: ls)),
+    cases h : (nxor.eval α (l :: ls)),
     { apply eval_ff_iff_exists_clause_eval_ff.mpr,
       use (clause.falsify α (map var (l :: ls))),
       split,
@@ -200,11 +171,24 @@ begin
         ((even_flips_iff_mem_direct_xor_of_map_var_eq mve).mpr hc) he.symm,
       have neq := ne_of_apply_ne nat.bodd neqodd,
       rw clause.count_flips_comm at neq,
-      exact clause.eval_tt_of_neq_flips mve.symm (ne.symm neq) } }
+      exact clause.eval_tt_of_ne_flips mve.symm (ne.symm neq) } }
+end
+
+-- The stronger statement of eval_direct_xor_eq_eval_nxor is sufficient
+theorem direct_xor_equisatisfiable (g : nxor V) :
+  assignment.eqsat (λ α, cnf.eval α (direct_xor g)) (λ α, g.eval α) :=
+begin
+  split,
+  { rintros ⟨α, ha⟩,
+    use α, simp at ha,
+    simp only [← eval_direct_xor_eq_eval_nxor, ha] },
+  { rintros ⟨α, ha⟩,
+    use α, simp at ha,
+    simp only [eval_direct_xor_eq_eval_nxor, ha] }
 end
 
 /-
-theorem vars_direct_xor (g : xor_gate V) : cnf.vars (direct_xor g) = vars g :=
+theorem vars_direct_xor (g : nxor V) : cnf.vars (direct_xor g) = vars g :=
 begin
   induction g with v vs ih,
   { simp only [cnf.vars_singleton, direct_xor_nil, vars_nil, clause.vars_nil] },
@@ -214,5 +198,4 @@ end
 
 end direct_encoding
 
-end xor_gate
-
+end nxor
